Complexitylib/Classes.lean
@@ -25,6 +25,7 @@ import Complexitylib.Classes.PPoly.Uniform.Unrolling.Generator.PolynomialOffset
 import Complexitylib.Classes.PPoly.Uniform.Unrolling.Generator.Primitive
 import Complexitylib.Classes.PPoly.Uniform.Unrolling.Generator.Program
 import Complexitylib.Classes.PPoly.Uniform.Unrolling.Generator.Transition.PackedCopy
+import Complexitylib.Classes.PPoly.Uniform.Unrolling.Generator.Transition.Predecessor
 import Complexitylib.Classes.PPoly.Uniform.Unrolling.Generator.Transition.Read
 import Complexitylib.Classes.PPoly.Uniform.Unrolling.Generator.Transition.Case
 import Complexitylib.Classes.PPoly.Uniform.Unrolling.Stream
